

Q8

$$f(x, y) = \frac{1}{2\pi\sigma^2} \exp\left\{-\frac{1}{2} \frac{x^2 + y^2}{\sigma^2}\right\}$$

$$F(a \leq x \leq b, c < y \leq d)$$

$$\frac{1}{2\pi\sigma^2} \int_c^d \left(\int_a^b \exp\left\{-\frac{1}{2} \frac{x^2 + y^2}{\sigma^2}\right\} dx \right) dy = \frac{1}{2\pi\sigma^2} \int_c^d \exp\left\{-\frac{1}{2} \frac{y^2}{\sigma^2}\right\} dy \int_a^b \exp\left\{-\frac{1}{2} \frac{x^2}{\sigma^2}\right\} dx$$

F(r)?

one way: use polar coordinates

instead of x, y , use $r = \sqrt{x^2 + y^2}$

inverse transformation: $\theta = \tan\left(\frac{y}{x}\right)$

$$x(r, \theta) = r \cos \theta$$

$$y(r, \theta) = r \sin \theta$$

Using change of variables: ↗

$$f_{r, \theta}(r, \theta) = f_x(\underbrace{x(r, \theta)}_{r \cos \theta}, \underbrace{y(r, \theta)}_{r \sin \theta}) \cdot |\det J(\theta, r)|$$

$$J = \begin{bmatrix} \frac{dx(r, \theta)}{dr} & \frac{dx(r, \theta)}{d\theta} \\ \frac{dy(r, \theta)}{dr} & \frac{dy(r, \theta)}{d\theta} \end{bmatrix} = \begin{bmatrix} \cos \theta & -r \sin \theta \\ \sin \theta & r \cos \theta \end{bmatrix}$$

$$|\det J| = |r \cos^2 \theta + r \sin^2 \theta| = r$$

$$\downarrow N(x, y | \begin{bmatrix} 0 \\ 0 \end{bmatrix}, \begin{bmatrix} \sigma^2 & 0 \\ 0 & \sigma^2 \end{bmatrix})$$

$$f_x(r \cos \theta, r \sin \theta) \cdot r$$

$$\frac{1}{2\pi \sigma^2} \exp\left(\frac{-r^2 [\cancel{\cos^2 \theta} + \cancel{\sin^2 \theta}]^{\rightarrow 1}}{2\sigma^2}\right) r$$

$$f_r(r) = \int_0^{2\pi} f_{\theta, r}(\theta, r) d\theta = \frac{1}{\sigma^2} \left(\exp\left\{-\frac{r^2}{2\sigma^2}\right\} \right) r$$

$$F_r(R) = \frac{1}{\sigma^2} \int_0^R r \exp\left(-\frac{1}{2\sigma^2} r^2\right) dr$$

primitive: $-\exp\left(-\frac{1}{2\sigma^2} r^2\right) + C$
of $f_r(r)$

check: $\frac{d(P)}{dr} = -\exp\left(-\frac{1}{2\sigma^2} r^2\right) \cdot -\frac{1}{\sigma^2} r$

$\frac{d(\text{primitive})}{dr}$ yields exactly the function $f_r(r)$

$$= -\exp\left(-\frac{1}{2\sigma^2} r^2\right) \Big|_0^R = 0 - 1$$

$$\Rightarrow P. \left[\text{CDF}(r) = 1 - \exp\left(-\frac{r^2}{2\sigma^2}\right) \right]$$

$C=1$ must be added to
ensure $\text{CDF}(\infty) = 1$
 $\text{CDF}(0) = 0$